IntroLean/Sheet6.lean
@@ -1,0 +1,59 @@
+import Mathlib.Tactic -- imports all of the tactics in Lean's maths library
+
+set_option autoImplicit false
+set_option tactic.hygienic false
+
+
+-- inductive predicate
+
+inductive IsSorted: List ℕ  → Prop
+  -- Base Case 1: The empty list is sorted.
+  | nil : IsSorted []
+  -- Base Case 2: A list with a single element is sorted.
+  | single (a : ℕ) : IsSorted [a]
+  -- Inductive Step: If we have an element `a` and another element `b`,
+  -- and a tail list `t`, then the list `a :: b :: t` is sorted if:
+  -- 1. `a` is less than or equal to `b` (`a ≤ b`).
+  -- 2. The rest of the list, `b :: t`, is already sorted.
+  | cons (a b : ℕ ) (t : List ℕ ) : a ≤ b → IsSorted (b :: t) → IsSorted (a :: b :: t)
+
+
+#check IsSorted [20, 3]      -- Output: Prop
+example: IsSorted [1] := by
+  exact IsSorted.single 1
+
+example: IsSorted [1,3] := by
+  apply IsSorted.cons
+  omega
+  apply IsSorted.single
+
+example: ¬ IsSorted [20,3] := by
+  by_contra!
+  cases this
+  absurd a_1
+  omega
+
+def Merge: List ℕ → List ℕ → List ℕ
+  | [],[] => []
+  | x, [] => x
+  | [], y => y
+  | x::xs, y::ys =>
+    if x ≤ y then x :: Merge xs (y::ys)
+    else y :: Merge (x :: xs) ys
+
+#check Merge
+
+def Merge' (xs ys : List ℕ):  List ℕ :=
+  match xs,ys with
+  | [],[] => []
+  | x, [] => x
+  | [], y => y
+  | x::xs, y::ys =>
+    if x ≤ y then x :: Merge xs (y::ys)
+    else y :: Merge (x :: xs) ys
+
+def list1 := [1,2,10]
+def list2 := [3,5,20]
+#eval Merge list1 list2
+
+theorem sorted_merge (xs ys : List ℕ)(hxs: IsSorted xs) (hys: IsSorted ys): IsSorted (Merge xs ys) := by sorry
